theories/Dot/fundamental.v
@@ -20,9 +20,9 @@ Section fundamental.
   Context `{!dlangG Σ} `{!SwapProp (iPropSI Σ)}.
   Context `{hasStampTable: stampTable}.
 
-  Lemma fundamental_dm_typed Γ V l d T (HT: Γ |d V ⊢{ l := d } : T):
+  Lemma fundamental_dm_typed Γ V l d T (HT: Γ |L V ⊢{ l := d } : T):
     Γ |L V ⊨[ ⟦ getStampTable ⟧g ] { l := d } : T with
-  fundamental_dms_typed Γ V ds T (HT: Γ |ds V ⊢ ds : T):
+  fundamental_dms_typed Γ V ds T (HT: Γ |L V ⊢ ds : T):
     Γ |L V ⊨[ ⟦ getStampTable ⟧g ]ds ds : T with
   fundamental_subtype Γ T1 i1 T2 i2 (HT: Γ ⊢ₜ T1, i1 <: T2, i2):
     Γ ⊨[ ⟦ getStampTable ⟧g ] T1, i1 <: T2, i2 with
